Error 117 발생? 순환 참조? - 이게 무슨 오류지;;

src/common/Nemonuri.IndexedStackMap.fst
@@ -15,6 +15,7 @@ private let rec create_indices_set_agg (n: nat) (idx:I.under (n+1)) :
 let create_indices_set (n: nat) : Tot (FSet.set (I.under n)) =
   create_indices_set_agg n 0
 
+let indexed_stack_map_predicate (#n:nat) (#data_t:Type) (m:FMap.map (I.under n) data_t) = FSet.equal (FMap.domain m) (create_indices_set n)
 
 open FStar.FiniteSet.Ambient
 open FStar.FiniteMap.Ambient
