src/common/Nemonuri.IndexedStackMap.fsti
@@ -6,8 +6,8 @@ module FSet = FStar.FiniteSet.Base
 
 val create_indices_set (n: nat) : Tot (FSet.set (I.under n))
 
-let indexed_stack_map_predicate (#n:nat) (#data_t:Type) (m:FMap.map (I.under n) data_t) =
-  FSet.equal (FMap.domain m) (create_indices_set n)
+val indexed_stack_map_predicate (#n:nat) (#data_t:Type) (m:FMap.map (I.under n) data_t) : Tot Type0
+  //FSet.equal (FMap.domain m) (create_indices_set n)
 
 val lemma_create_indices_set_zero () : Lemma (ensures FSet.equal (FSet.emptyset) (create_indices_set 0))
 
